began with receiver cont proof

CaseStudies/ABP/ABP_TSPS.thy
@@ -53,6 +53,12 @@ abbreviation invBool :: "'a MABP \<Rightarrow> bool" where
 
 abbreviation invData :: "'a MABP \<Rightarrow> 'a" where
 "invData \<equiv> (inv Data)"
+
+abbreviation recvAbb where
+"recvAbb \<equiv> 
+let recRes = (\<lambda> x. tsRec\<cdot>((tsMap invBoolPair)\<cdot>(x . dr)))
+in (\<lambda> x. (tsbDom\<cdot>x = {dr}) \<leadsto> [ar    \<mapsto> tsMap Bool\<cdot>(fst (recRes x)),
+                                        abpOut \<mapsto> tsMap Data\<cdot>(snd (recRes x))]\<Omega>)" 
   
 
 subsection \<open>receiver\<close> 
@@ -61,7 +67,22 @@ definition recvTSPF :: "'a MABP TSPF" where
 let recRes = (\<lambda> x. tsRec\<cdot>((tsMap invBoolPair)\<cdot>(x . dr)))
 in Abs_CTSPF (\<lambda> x. (tsbDom\<cdot>x = {dr}) \<leadsto> [ar    \<mapsto> tsMap Bool\<cdot>(fst (recRes x)),
                                         abpOut \<mapsto> tsMap Data\<cdot>(snd (recRes x))]\<Omega>)"
+
+subsection \<open>medium_rs\<close>
+  (* medium from receiver to sender *)
+  (* input: ar, output: as, transport booleans *)
   
+definition tsMedRSTSPF :: "bool stream \<Rightarrow> 'a MABP TSPF" where
+"tsMedRSTSPF bst\<equiv> Abs_CTSPF (\<lambda> x. (tsbDom\<cdot>x = {ar}) 
+                                    \<leadsto> [as \<mapsto> tsMap Bool\<cdot>(tsMed\<cdot>(tsMap invBool\<cdot>(x . ar))\<cdot>bst)]\<Omega>)"
+  
+subsection \<open>medium_sr\<close>
+  (* medium from sender to receiver *)
+  (* input: ds, output: dr, transport (data, bool) tuples *)
+  
+definition tsMedSRTSPF :: "bool stream \<Rightarrow> 'a MABP TSPF" where
+"tsMedSRTSPF bst\<equiv> Abs_CTSPF (\<lambda> x. (tsbDom\<cdot>x = {ds}) 
+                                \<leadsto> [dr \<mapsto> tsMap BoolPair\<cdot>(tsMed\<cdot>(tsMap invBoolPair\<cdot>(x . ds))\<cdot>bst)]\<Omega>)"
 
 
 (* ----------------------------------------------------------------------- *)
@@ -89,20 +110,176 @@ lemma data_data_inv [simp]: "(inv Data) (Data x) = x"
   by (meson MABP.inject(3) f_inv_into_f rangeI)
   
 
+subsection \<open>receiver\<close>
 
-lemma "(\<lambda> x. if x= Bool True then True else False) (Bool False) = False"
-  by simp
-    
-lemma "(\<lambda> x. THE b. x = (Bool b)) (Bool x) = x"
-  by (simp add: the_equality)
+lemma "cont (\<lambda> x. tsMap Bool\<cdot>(fst (tsRec\<cdot>((tsMap invBoolPair)\<cdot>(x .dr)))))"
+  by (simp add: monofun_fst)
   
-lemma "(inv Bool) (Bool x) = x"
-  by (meson MABP.inject(2) f_inv_into_f rangeI) 
+lemma "x \<sqsubseteq> y \<Longrightarrow> tsMap Bool\<cdot>(fst (tsRec\<cdot>(tsMap invBoolPair\<cdot>(x  .  dr)))) \<sqsubseteq> tsMap Bool\<cdot>(fst (tsRec\<cdot>(tsMap invBoolPair\<cdot>(y  .  dr))))"
+  by (simp add: fst_monofun monofun_cfun_arg tsbgetch_below)
+
+definition testf :: "'a MABP TSB \<Rightarrow> 'a MABP tstream"  where
+  "testf \<equiv> (\<lambda> x. tsMap Bool\<cdot>(fst (tsRec\<cdot>((tsMap invBoolPair)\<cdot>(x .dr)))))"
     
-lemma "(inv Data) (Data x) = x"
-  by (meson MABP.inject(3) f_inv_into_f rangeI)
+lemma f21: assumes "  chain Y" and "tsbDom\<cdot>(\<Squnion>i::nat. Y i) = {dr}"
+  shows "testf ((\<Squnion>i. Y i)) = (\<Squnion>i. (testf ((Y i))))"
+  apply (rule cont2contlubE)
+  by (simp_all add: assms testf_def)
+
+lemma testme: "tsMap Bool\<cdot>(fst (tsRec\<cdot>((tsMap invBoolPair)\<cdot>(x .dr)))) = (testf::'a MABP TSB \<Rightarrow> 'a MABP tstream) x"
+  by (simp add: testf_def)
+  
+(*
+lemma assumes "  chain Y" and "tsbDom\<cdot>(\<Squnion>i::nat. Y i) = {dr}"
+  shows "tsMap Bool\<cdot>(fst (tsRec\<cdot>(tsMap invBoolPair\<cdot>((\<Squnion>i. Y i)  .  dr)))) \<sqsubseteq> (\<Squnion>i::nat. tsMap Bool\<cdot>(fst (tsRec\<cdot>(tsMap invBoolPair\<cdot>(Y i  .  dr)))))"
+proof -
+  have f1: "tsMap Bool\<cdot>(fst (tsRec\<cdot>(tsMap invBoolPair\<cdot>((\<Squnion>i. Y i)  .  dr)))) = testf ((\<Squnion>i. Y i)) "
+    by (simp add: testf_def)
+  have f2: "(\<Squnion>i::nat. tsMap Bool\<cdot>(fst (tsRec\<cdot>(tsMap invBoolPair\<cdot>(Y i  .  dr))))) = (\<Squnion>i. (testf ((Y i))))"
+    by (simp add: testf_def)
+  show ?thesis
+   apply (subst testme)
+      
+ 
+  
+lemma "monofun (\<lambda> x.  tsMap Bool\<cdot>(fst (tsRec\<cdot>(x))))" 
+  apply (rule monofunI)
+    oops
+*)
     
+lemma recv_tsb_well [simp]:
+  shows "tsb_well [ar \<mapsto> tsMap Bool\<cdot>(fst (tsRec\<cdot>((tsMap invBoolPair)\<cdot>(x . dr)))),
+                                    abpOut \<mapsto> tsMap Data\<cdot>(snd (tsRec\<cdot>((tsMap invBoolPair)\<cdot>(x . dr))))]"
+  apply (rule tsb_wellI)
+  apply (simp add: tsmap_tsdom_range)
+  by blast
+    
+lemma recv_tsb_dom: "tsbDom\<cdot>( [ar \<mapsto> tsMap Bool\<cdot>(fst (tsRec\<cdot>((tsMap invBoolPair)\<cdot>(x . dr)))),
+                                    abpOut \<mapsto> tsMap Data\<cdot>(snd (tsRec\<cdot>((tsMap invBoolPair)\<cdot>(x . dr))))]\<Omega>) = {ar, abpOut}"
+  apply (simp add: tsbdom_rep_eq)
+    by auto
+ 
+lemma rec_tsb_mono: "\<And>(x::'a MABP TSB) y::'a MABP TSB. tsbDom\<cdot>x = {dr} \<Longrightarrow> x \<sqsubseteq> y \<Longrightarrow> 
+          [ar \<mapsto> tsMap Bool\<cdot>(fst (tsRec\<cdot>(tsMap invBoolPair\<cdot>(x  .  dr)))), 
+          abpOut \<mapsto> tsMap Data\<cdot>(snd (tsRec\<cdot>(tsMap invBoolPair\<cdot>(x  .  dr))))]\<Omega> 
+          \<sqsubseteq> [ar \<mapsto> tsMap Bool\<cdot>(fst (tsRec\<cdot>(tsMap invBoolPair\<cdot>(y  .  dr)))), 
+             abpOut \<mapsto> tsMap Data\<cdot>(snd (tsRec\<cdot>(tsMap invBoolPair\<cdot>(y  .  dr))))]\<Omega>"
+      apply (rule tsb_below)
+       apply (simp_all add: tsbdom_below tsbdom_rep_eq tsbgetch_rep_eq)
+       by (simp add: fst_monofun snd_monofun monofun_cfun_arg tsbgetch_below)
+     
   
+lemma recvTSPF_mono [simp]: "monofun (\<lambda> x. (tsbDom\<cdot>x = {dr}) \<leadsto> [ar \<mapsto> tsMap Bool\<cdot>(fst (tsRec\<cdot>((tsMap invBoolPair)\<cdot>(x . dr)))),
+                                        abpOut \<mapsto> tsMap Data\<cdot>(snd (tsRec\<cdot>((tsMap invBoolPair)\<cdot>(x . dr))))]\<Omega>)"
+  apply (rule tspf_monoI)
+  apply (rule tsb_below)
+   apply (simp_all add: tsbdom_below tsbdom_rep_eq tsbgetch_rep_eq)
+   by (simp add: fst_monofun snd_monofun monofun_cfun_arg tsbgetch_below)
   
+     
+lemma recvTSPF_tsb_getc: assumes "chain Y" and "tsbDom\<cdot>(\<Squnion>i. Y i) = {dr}"
+  and "c \<in>  {ar, abpOut}"
+  shows " (\<Squnion>i.
+           [ar \<mapsto> tsMap Bool\<cdot>(fst (tsRec\<cdot>(tsMap invBoolPair\<cdot>(Y i  .  dr)))), abpOut \<mapsto>
+            tsMap Data\<cdot>(snd (tsRec\<cdot>(tsMap invBoolPair\<cdot>(Y i  .  dr))))]\<Omega>) . c
+          = (\<Squnion> i. ([ar \<mapsto> tsMap Bool\<cdot>(fst (tsRec\<cdot>(tsMap invBoolPair\<cdot>(Y i  .  dr)))), abpOut \<mapsto>
+            tsMap Data\<cdot>(snd (tsRec\<cdot>(tsMap invBoolPair\<cdot>(Y i  .  dr))))]\<Omega>) . c)"
+proof (rule lubgetCh)
+   have f2: "\<And> i. tsbDom\<cdot>(Y i) =  tsbDom\<cdot>(\<Squnion>i. Y i)"
+     by (simp add: assms(1))
+   show tb_chain: "chain (\<lambda>i::nat. [ar \<mapsto> tsMap Bool\<cdot>(fst (tsRec\<cdot>(tsMap invBoolPair\<cdot>(Y i  .  dr)))), abpOut \<mapsto>
+                      tsMap Data\<cdot>(snd (tsRec\<cdot>(tsMap invBoolPair\<cdot>(Y i  .  dr))))]\<Omega>)"
+     by (simp add: assms(1) assms(2) po_class.chainE po_class.chainI rec_tsb_mono)
+   
+   show " c \<in> tsbDom\<cdot>(\<Squnion>i::nat. [ar \<mapsto> tsMap Bool\<cdot>(fst (tsRec\<cdot>(tsMap invBoolPair\<cdot>(Y i  .  dr)))), abpOut \<mapsto>
+                           tsMap Data\<cdot>(snd (tsRec\<cdot>(tsMap invBoolPair\<cdot>(Y i  .  dr))))]\<Omega>)"
+     using assms(3) recv_tsb_dom tb_chain tsbChain_dom_eq2 by blast
+qed
+   
+     
+
+  
+lemma recvTSPF_cont: "cont (\<lambda> x. (tsbDom\<cdot>x = {dr}) \<leadsto> [ar \<mapsto> tsMap Bool\<cdot>(fst (tsRec\<cdot>((tsMap invBoolPair)\<cdot>(x . dr)))),
+                                        abpOut \<mapsto> tsMap Data\<cdot>(snd (tsRec\<cdot>((tsMap invBoolPair)\<cdot>(x . dr))))]\<Omega>)"
+  proof (rule tspf_contI)
+  
+    show recv_mono: "\<And>(x::'a MABP TSB) y::'a MABP TSB. tsbDom\<cdot>x = {dr} \<Longrightarrow> x \<sqsubseteq> y \<Longrightarrow> 
+          [ar \<mapsto> tsMap Bool\<cdot>(fst (tsRec\<cdot>(tsMap invBoolPair\<cdot>(x  .  dr)))), 
+          abpOut \<mapsto> tsMap Data\<cdot>(snd (tsRec\<cdot>(tsMap invBoolPair\<cdot>(x  .  dr))))]\<Omega> 
+          \<sqsubseteq> [ar \<mapsto> tsMap Bool\<cdot>(fst (tsRec\<cdot>(tsMap invBoolPair\<cdot>(y  .  dr)))), 
+             abpOut \<mapsto> tsMap Data\<cdot>(snd (tsRec\<cdot>(tsMap invBoolPair\<cdot>(y  .  dr))))]\<Omega>"
+      by (simp add: rec_tsb_mono)
+      
+    have f1: " \<And>Y::nat \<Rightarrow> 'a MABP TSB. chain Y \<Longrightarrow> tsbDom\<cdot>(\<Squnion>i::nat. Y i) = {dr} \<Longrightarrow> 
+                tsbDom\<cdot>(\<Squnion>i::nat. [ar \<mapsto> tsMap Bool\<cdot>(fst (tsRec\<cdot>(tsMap invBoolPair\<cdot>(Y i  .  dr)))), 
+                abpOut \<mapsto> tsMap Data\<cdot>(snd (tsRec\<cdot>(tsMap invBoolPair\<cdot>(Y i  .  dr))))]\<Omega>) = {abpOut, ar}"
+     proof -
+      fix Y :: "nat \<Rightarrow> 'a MABP TSB"
+      assume a1: "chain Y"
+      assume a2: "tsbDom\<cdot>(\<Squnion>i. Y i) = {dr}"
+      have f3: "\<forall>t ta. (tsbDom\<cdot>t \<noteq> {dr} \<or> t \<notsqsubseteq> ta) \<or> [ar \<mapsto> tsMap Bool\<cdot> (fst (tsRec\<cdot>(tsMap invBoolPair\<cdot>(t . dr)))), abpOut \<mapsto> tsMap Data\<cdot> (snd (tsRec\<cdot> (tsMap invBoolPair\<cdot> (t . dr)))::'a tstream)]\<Omega> \<sqsubseteq> [ar \<mapsto> tsMap Bool\<cdot> (fst (tsRec\<cdot>(tsMap invBoolPair\<cdot>(ta . dr)))), abpOut \<mapsto> tsMap Data\<cdot> (snd (tsRec\<cdot>(tsMap invBoolPair\<cdot>(ta . dr))))]\<Omega>"
+        using recv_mono by blast
+      have f4: "\<forall>f n. \<not> chain f \<or> tsbDom\<cdot>(f n::'a MABP TSB) = tsbDom\<cdot>(Lub f)"
+        by (meson tsbChain_dom_eq2)
+      have f5: "\<And> elem_1 .tsbDom\<cdot> ([ar \<mapsto> tsMap Bool\<cdot> (fst (tsRec\<cdot>(tsMap invBoolPair\<cdot>(Y elem_1 . dr)))), abpOut \<mapsto> tsMap Data\<cdot> (snd (tsRec\<cdot> (tsMap invBoolPair\<cdot>(Y elem_1 . dr))))]\<Omega>) = {ar, abpOut}"
+        by (simp add: recv_tsb_dom)
+      have "\<And> v1_0. tsbDom\<cdot> (Y (v1_0 (\<lambda>n. [ar \<mapsto> tsMap Bool\<cdot> (fst (tsRec\<cdot>(tsMap invBoolPair\<cdot>(Y n . dr)))), abpOut \<mapsto> tsMap Data\<cdot> (snd (tsRec\<cdot> (tsMap invBoolPair\<cdot>(Y n . dr))))]\<Omega>))) = {dr}"
+        using f4 a2 a1 by presburger
+      then have "chain (\<lambda>n. [ar \<mapsto> tsMap Bool\<cdot> (fst (tsRec\<cdot>(tsMap invBoolPair\<cdot>(Y n . dr)))), abpOut \<mapsto> tsMap Data\<cdot> (snd (tsRec\<cdot>(tsMap invBoolPair\<cdot>(Y n . dr))))]\<Omega>)"
+        using f3 a1 by (simp add: po_class.chain_def)
+      then show "tsbDom\<cdot> (\<Squnion>n. [ar \<mapsto> tsMap Bool\<cdot> (fst (tsRec\<cdot>(tsMap invBoolPair\<cdot>(Y n . dr)))), abpOut \<mapsto> tsMap Data\<cdot> (snd (tsRec\<cdot>(tsMap invBoolPair\<cdot>(Y n . dr))))]\<Omega>) = {abpOut, ar}"
+        using f5 f4 by blast
+    qed
+      
+    (* maybe has to do with fixation and the type of the receiver *)
+   have f3: "\<And>(Y::nat \<Rightarrow> 'a MABP TSB) c::channel. chain Y \<Longrightarrow> tsbDom\<cdot>(\<Squnion>i::nat. Y i) = {dr} \<Longrightarrow> c = ar \<or> c = abpOut \<Longrightarrow> c = ar \<longrightarrow> tsMap Bool\<cdot>(fst (tsRec\<cdot>(tsMap invBoolPair\<cdot>(Lub Y  .  dr)))) \<sqsubseteq> (\<Squnion>i::nat. tsMap Bool\<cdot>(fst (tsRec\<cdot>(tsMap invBoolPair\<cdot>(Y i  .  dr)))))"
+     sorry
+       
+   have f4: "\<And>(Y::nat \<Rightarrow> 'a MABP TSB) c::channel. chain Y \<Longrightarrow> tsbDom\<cdot>(\<Squnion>i::nat. Y i) = {dr} \<Longrightarrow> c = ar \<or> c = abpOut \<Longrightarrow> c = ar \<longrightarrow>  tsMap Data\<cdot>(snd (tsRec\<cdot>(tsMap invBoolPair\<cdot>(Lub Y  .  dr)))) \<sqsubseteq> (\<Squnion>i::nat. tsMap Data\<cdot>(snd (tsRec\<cdot>(tsMap invBoolPair\<cdot>(Y i  .  dr)))))"
+     sorry
+       
+    show "\<And>Y::nat \<Rightarrow> 'a MABP TSB.
+       chain Y \<Longrightarrow>
+       tsbDom\<cdot>(\<Squnion>i::nat. Y i) = {dr} \<Longrightarrow>
+       [ar \<mapsto> tsMap Bool\<cdot>(fst (tsRec\<cdot>(tsMap invBoolPair\<cdot>((\<Squnion>i::nat. Y i)  .  dr)))), abpOut \<mapsto>
+        tsMap Data\<cdot>(snd (tsRec\<cdot>(tsMap invBoolPair\<cdot>((\<Squnion>i::nat. Y i)  .  dr))))]\<Omega> \<sqsubseteq>
+       (\<Squnion>i::nat.
+           [ar \<mapsto> tsMap Bool\<cdot>(fst (tsRec\<cdot>(tsMap invBoolPair\<cdot>(Y i  .  dr)))), abpOut \<mapsto>
+            tsMap Data\<cdot>(snd (tsRec\<cdot>(tsMap invBoolPair\<cdot>(Y i  .  dr))))]\<Omega>)"
+      apply (rule tsb_below)
+       apply (simp_all add: tsbdom_below tsbdom_rep_eq tsbgetch_rep_eq f1)
+      apply (simp add: recvTSPF_tsb_getc tsbdom_rep_eq tsbgetch_rep_eq)
+      using f3 f4 by fastforce
+  qed
+    
+        
+        
+       
+    
+    
+    
+    
+    
+    
+    
+    
+    
+    
+    
+    
+    
+    
+    
+    
+    
+    
+    
+    
+    
+    
+    
+    
+    
+    
     
 end
